src/reordering/ReorderingMapper.v
@@ -145,6 +145,17 @@ Proof using.
   now apply rsr_mapper_tid'.
 Qed.
 
+Lemma rsr_mapper_sametid e s
+    (TID : tid a_t = tid b_t) :
+  mapper ↑₁ (s ∩₁ same_tid e) ≡₁
+    mapper ↑₁ s ∩₁ same_tid e.
+Proof using.
+  unfolder. split; ins; desf.
+  all: eexists; splits; eauto.
+  all: unfold same_tid in *.
+  all: rewrite rsr_mapper_tid' in *; auto.
+Qed.
+
 Lemma rsr_mapper_inj
     (NEQ : a_t <> b_t) :
   inj_dom ⊤₁ mapper.
@@ -289,6 +300,15 @@ Proof using.
   all: auto with hahn.
 Qed.
 
+Lemma rsr_mapper_init
+    (ANIN : ~is_init a_t)
+    (BNIN : ~is_init b_t) :
+  fixset is_init mapper.
+Proof using.
+  unfolder. ins.
+  rewrite rsr_mappero; congruence.
+Qed.
+
 End ReordMapper.
 
 #[global]
@@ -296,4 +316,4 @@ Hint Resolve rsr_mapper_at rsr_mapper_bt
   rsr_mappero rsr_mapper_tid rsr_mapper_inj
   rsr_mapper_inv_at rsr_mapper_bt
   rsr_mapper_tid' rsr_mapper_tid
-  rsr_mapper_self_inv : xmm.
+  rsr_mapper_self_inv rsr_mapper_init : xmm.
